Typecheck and fix logging code

src/go_lang/examples/logging.v
@@ -19,20 +19,35 @@ Module log.
   Definition logS := mkStruct ["log_sz"; "disk_sz"].
   Definition T: ty := intT * intT.
   Section fields.
-    Context {ext:ext_op}.
+    Context `{ext_ty:ext_types}.
     Definition log_sz := structF! logS "log_sz".
     Definition disk_sz := structF! logS "disk_sz".
+    Theorem log_sz_t Γ : Γ ⊢ log_sz : (T -> intT).
+    Proof.
+      typecheck.
+    Qed.
+    Theorem disk_sz_t Γ : Γ ⊢ disk_sz : (T -> intT).
+    Proof.
+      typecheck.
+    Qed.
   End fields.
 End log.
+
+Hint Resolve log.log_sz_t log.disk_sz_t : types.
 
 Import log.
 
 Definition write_hdr: val :=
   λ: "log",
     let: "hdr" := NewByteSlice #4096 in
-    UInt64Put "log_sz" "hdr";;
-    UInt64Put "disk_sz" ("hdr" +ₗ #8);;
+    UInt64Put (log_sz "log") "hdr";;
+    UInt64Put (disk_sz "log") (SliceSkip "hdr" #8);;
     Write #0 "hdr".
+
+Theorem write_hdr_t Γ : Γ ⊢ write_hdr : (T -> unitT).
+Proof.
+  typecheck.
+Qed.
 
 Definition init: val :=
   λ: "disk_sz",
@@ -42,6 +57,11 @@ Definition init: val :=
     write_hdr "log";;
     ("log", #true).
 
+Theorem init_t Γ : Γ ⊢ init : (intT -> T * boolT).
+Proof.
+  typecheck.
+Qed.
+
 Definition get: val :=
   λ: "log" "i",
   let: "sz" := log.log_sz "log" in
@@ -49,12 +69,24 @@ Definition get: val :=
   then (Read (#1+"i"), #true)
   else (slice.nil, #false).
 
+Theorem get_t Γ : Γ ⊢ get : (T -> intT -> slice.T byteT * boolT).
+Proof.
+  typecheck.
+Qed.
+
 Definition write_all: val :=
   λ: "bks" "off",
   let: "len" := slice.len "bks" in
   for: "i" < "len" :=
     let: "bk" := SliceGet "bks" "i" in
     Write ("off" + "i") "bk".
+
+Theorem write_all_t Γ : Γ ⊢ write_all : (slice.T (slice.T byteT) -> intT -> unitT).
+Proof.
+  typecheck.
+Qed.
+
+Hint Resolve write_all_t : types.
 
 Definition append: val :=
   λ: "logp" "bks",
@@ -69,17 +101,32 @@ Definition append: val :=
     "logp" <- "new_log";;
     #true.
 
+Theorem append_t Γ : Γ ⊢ append : (refT T -> slice.T (slice.T byteT) -> boolT).
+Proof.
+  typecheck.
+Qed.
+
 Definition reset: val :=
   λ: "logp",
-  let: "new_log" := (#0, log.disk_sz !"log") in
+  let: "new_log" := (#0, log.disk_sz !"logp") in
   write_hdr "new_log";;
   "logp" <- "new_log";;
   #().
 
+Theorem reset_t Γ : Γ ⊢ reset : (refT T -> unitT).
+Proof.
+  typecheck.
+Qed.
+
 Definition recover: val :=
   λ: <>,
      let: "hdr" := Read #0 in
-     let: "log_sz" := UInt64Get ("hdr", #8) in
-     let: "disk_sz" := UInt64Get (("hdr" +ₗ #8), #8) in
+     let: "log_sz" := UInt64Get (SliceTake "hdr" #8) in
+     let: "disk_sz" := UInt64Get (SliceTake (SliceSkip "hdr" #8) #8) in
      let: "log" := ("log_sz", "disk_sz") in
      "log".
+
+Theorem recover_t Γ : Γ ⊢ recover : (unitT -> T).
+Proof.
+  typecheck.
+Qed.
